Battteries/Vector/Lemmas.lean
@@ -1,8 +1,31 @@
 
-import Batteries.Data.Vector.Lemmas
-import Battteries.List.Lemmas
+-- import Batteries.Data.Vector.Lemmas
+-- import Battteries.List.Lemmas
 
-namespace Batteries.Vector
+private theorem List.exists_three_of_le (l : List α) (h1 : i ≤ j) (h2 : j ≤ l.length) :
+    ∃ l₁ l₂ l₃, l₁.length = i ∧ i + l₂.length = j ∧ l = l₁ ++ l₂ ++ l₃ := by
+
+  let exists_of_length_le {n} {l : List α} (h : n ≤ l.length) :
+      ∃ l₁ l₂, l = l₁ ++ l₂ ∧ l₁.length = n :=
+    ⟨_, _, (List.take_append_drop n l).symm, List.length_take_of_le h⟩
+
+  obtain ⟨l', l₃, rfl, rfl⟩ := exists_of_length_le h2
+  let ⟨l₁, l₂, eq, hl₁⟩ := exists_of_length_le h1
+  exact ⟨l₁, l₂, l₃, hl₁, by simp [eq, hl₁]⟩
+
+
+theorem Vector.split_three (as : Vector α n) (h1 : lo ≤ hi) (h2 : hi ≤ n) :
+    ∃ (L₁ L₂ L₃ : List α), (L₁.length = lo) ∧ (lo + L₂.length = hi) ∧
+      (as.1.toList = L₁ ++ L₂ ++ L₃) :=
+  have : hi ≤ as.toArray.size := as.2.symm ▸ h2
+  List.exists_three_of_le _ h1 (show hi ≤ as.toArray.toList.length from this)
+
+
+-- #check Vector
+
+
+
+-- namespace Vector
 
 -- -- TODO: (@somombo) add this instance upstream?
 -- instance : CoeOut (Vector α n) (Array α) where
@@ -10,24 +33,25 @@ namespace Batteries.Vector
 
 
 -- TODO: @somombo add these to Vectors API
-@[simp] theorem getElem_swap_right (a : Vector α n) {i j : Fin n} : (a.swap i j)[j.val] = a[i] := a.1.getElem_swap_right
+#check _root_.Vector.getElem_swap_of_ne
+-- @[simp] theorem getElem_swap_right (a : Vector α n) {i j : Fin n} : (a.swap i j)[j.val] = a[i] := a.1.getElem_swap_right
 
-@[simp] theorem getElem_swap_left (a :  Vector α n) {i j : Fin n} : (a.swap i j)[i.val] = a[j] := a.1.getElem_swap_left
+-- @[simp] theorem getElem_swap_left (a :  Vector α n) {i j : Fin n} : (a.swap i j)[i.val] = a[j] := a.1.getElem_swap_left
 
-@[simp] theorem getElem_swap_of_ne (a : Vector α n) {i j : Fin n} (hp : p < n)
-    (hi : p ≠ i) (hj : p ≠ j) : (a.swap i j)[p] = a[p] := a.1.getElem_swap_of_ne (a.2.symm ▸ hp) hi hj
+-- @[simp] theorem getElem_swap_of_ne (a : Vector α n) {i j : Fin n} (hp : p < n)
+--     (hi : p ≠ i) (hj : p ≠ j) : (a.swap i j)[p] = a[p] := a.1.getElem_swap_of_ne (a.2.symm ▸ hp) hi hj
 
-theorem getElem_swap (a : Vector α n) (i j : Fin n) (k : Nat) (hk : k < n) :
-    (a.swap i j)[k] = if k = i then a[j] else if k = j then a[i] else a[k] :=
-  a.1.getElem_swap' (i.cast a.2.symm) (j.cast a.2.symm) k (a.2.symm ▸ hk)
 
-@[simp] theorem swap_self (a : Vector α n) {i : Fin n} : a.swap i i = a := by
-  apply Vector.ext
-  intros; simp only [getElem_swap]
-  split <;> simp_all
+#check Vector.getElem_swap
 
-theorem split_three (as : Vector α n) (h1 : lo ≤ hi) (h2 : hi ≤ n) :
-    ∃ (L₁ L₂ L₃ : List α), (L₁.length = lo) ∧ (lo + L₂.length = hi) ∧
-      (as.1.toList = L₁ ++ L₂ ++ L₃) :=
-  have : hi ≤ as.toArray.size := as.2.symm ▸ h2
-  List.exists_three_of_le _ h1 (show hi ≤ as.toArray.toList.length from this)
+-- @[grind]
+-- theorem getElem_swap'' {xs : Vector α n} {i j : Nat} (hi hj) {k : Nat} (hk : k < n) :
+--     (xs.swap i j hi hj)[k] = if k = i then xs[j] else if k = j then xs[i] else xs[k] := by
+--   cases xs
+--   simp_all [Array.getElem_swap]
+
+
+-- theorem getElem_swap (a : Vector α n) (i j : Fin n) (k : Nat) (hk : k < n) :
+--     (a.swap i j)[k] = if k = i then a[j] else if k = j then a[i] else a[k] :=
+--   a.1.getElem_swap' (i.cast a.2.symm) (j.cast a.2.symm) k (a.2.symm ▸ hk)
+-- end Vector
