Quicksort/Partition/Hoare/New/Basic.lean
@@ -1,0 +1,138 @@
+import Quicksort.Partition.Init.Basic
+
+namespace Partition
+
+variable [Ord α]
+
+-- instance : Nonempty ([Ord α] → {n j : Nat} → α → Vector α n → (jval : Nat) → jval ≤ j → j < n →
+--     { j' : Fin n // j' ≤ j }) :=
+--   ⟨fun _ _ jval hjj hj => ⟨⟨jval, by omega⟩, by grind⟩⟩
+
+
+
+def hoare.new.loop.while_j' (pivot : α)  (arr : Vector α n) (jval : Nat)  (hjj : jval ≤ j)
+    (hxj : left ≤ jval) (hj : j < n) : { j' : Nat // j' ≤ j }:=
+  if h' : jval = left ∨ lt arr[jval] pivot then
+    ⟨jval, by grind⟩
+  else
+    -- have _ : jval ≠ left := sorry
+    while_j' (left:=left) pivot  arr (jval - 1) (by omega) (by omega) (by omega)
+-- partial_fixpoint
+-- termination_by jval
+-- decreasing_by
+--   have hterm_strong_precon : ∃ (left : Nat) (hj' : left < n), left ≤ jval ∧ ¬ lt pivot arr[left] := sorry
+--   grind
+
+def hoare.new.loop.while_i' (pivot : α)  (arr : Vector α n) (ival : Nat) (hli : left < ival) (hxi : ival ≤ right)
+    (hr : right < n)  : { i' : Nat // left < i' } :=
+  -- NOTEvv: @somombo: ival = right → lt pivot arr[ival] if lt is asymmetric
+  if _ : ival = right ∨ lt pivot arr[ival] then
+    ⟨ival, hli⟩
+  else
+    -- have _ : ival ≠ right := sorry
+    while_i' (right:=right) pivot  arr (ival + 1)  (by omega) (by omega) hr
+
+
+open Vector in
+def hoare.new (arr : Vector α n) (left : Nat) (right : Nat) (hlr : left < right)
+    (hr : right < n) : { x : Partition α n  // left < x.i' ∧ x.j' < right } :=
+  have hl : left < n := by omega
+
+  let rec loop (pivot : α) (arr : Vector α n) (i j : Nat) /- (hj : j < n) -/ (hli : left < i)
+      (hir : i ≤ right) (hlj : left ≤ j) (hjr : j < right) : { x : Partition α n  // left < x.i' ∧ x.j' < right } :=
+
+    let ⟨j', _⟩ := new.loop.while_j' pivot  arr j  Nat.le.refl hlj (by omega)
+    let ⟨i', _⟩ := new.loop.while_i' pivot  arr i  hli hir hr
+
+    if _ : i' < j' then
+      let arr' := arr.swap i' j'
+      loop pivot arr' (i' + 1) (j' - 1) (by grind)  (by grind) (by grind) (by grind)
+    else if _ : j' < i' then
+      ⟨⟨arr, j', i'⟩, by grind, by grind⟩
+    else
+      ⟨⟨arr, j' - 1, i' + 1⟩, by grind, by grind⟩
+  -- termination_by j + 1 - i
+  -- decreasing_by
+  --   change j' - 1 + 1 - (i' + 1) < j + 1 - i
+  --   -- have hii__ : i ≤ i' := sorry
+  --   omega
+  -- partial_fixpoint
+
+  let mid := left + ((right - left)/2)
+  have hm : mid < n := by omega
+  let arr_ := arr
+    |> (maybeSwap · ⟨left, hl⟩ ⟨mid, hm⟩)
+    |> (maybeSwap · ⟨left, hl⟩ ⟨right, hr⟩)
+    |> (maybeSwap · ⟨mid, hm⟩ ⟨right, hr⟩)
+
+  let pivot := arr_[mid]
+  loop pivot arr_ (left + 1) (right - 1) (by omega) (by omega) (by omega) (by omega)
+
+
+
+
+
+
+
+
+
+
+
+
+
+
+
+
+
+
+
+
+
+
+
+
+
+
+
+
+-- theorem hoare.new.loop.while_j'_lt_n
+--     {pivot : α} {arr : Vector α n}
+--     -- (hterm_strong_precon : ∃ (left : Nat) (hj' : left < n), left ≤ jval ∧ ¬ lt pivot arr[left])
+--     :
+--     while_j' pivot arr jval hj < n := by
+--   unfold while_j'
+--   if h' : lt pivot arr[jval] then
+--     simp [h']
+--     apply while_j'_lt_n
+--     -- grind
+--   else
+--     grind
+-- termination_by jval
+-- decreasing_by
+--   rename_i e this a ; clear _x this a
+--   simp_all
+--   grind
+
+
+
+-- theorem hoare.new.loop.while_j'_ltj
+--     {left right : Nat} {hr : right < n} {hl : left < n} {pivot : α}
+--     {arr : Vector α n} {i j : Nat} {hjr : j < right} {hli : left < i}
+--     {jval : Nat} (hj : jval < n) (hxj : left ≤ jval) (hjj : jval ≤ j)
+
+--     -- {pivot : α} {arr : Vector α n}
+--     (hterm_strong_precon : ¬ lt pivot arr[left]) :
+--     while_j' pivot arr jval hj ≤ j := by
+--   unfold while_j'
+--   if h' : lt pivot arr[jval] then
+--     simp_all [-hterm_strong_precon]
+
+--     have _ : jval ≠ left := /- by omega -/
+--       (h' |> show ¬lt pivot arr[jval] by simpa only [·])
+--     exact while_j'_ltj (left:=left) (right:=right) (pivot:=pivot) (arr:=arr) (hli:=by omega) (hjr:=by omega) (hl:=by omega) (hr:=by omega)
+--       (jval:=jval-1) (hj:= by omega)
+--       (by grind) (by omega) (by grind)
+--   else
+--     simp [*]
+-- -- termination_by jval
+-- -- decreasing_by grind
